extract/Extract.v
@@ -202,6 +202,7 @@ Extract Inlined Constant errst_assoc => "".
 Extract Inlined Constant errst_assoc5 => "".
 Extract Inlined Constant errst_congr1 => "". (*TODO: make sure OK*)
 Extract Inlined Constant errst_bind_dep => "(fun x y -> y x () ())".
+Extract Inlined Constant errst_bind_dep' => "(fun x y -> y () x ())".
 
 
 (*Mutable state monads*)
