src/coqutil/CoqCtr.v
@@ -1,6 +1,6 @@
 (*A counter, mutable when extracted to OCaml.
   We put it in a module so that multiple instances can be created*)
-Require Import State.
+Require Import State StateHoareMonad.
 Import MonadNotations. 
 Local Open Scope state_scope.
 
@@ -8,6 +8,17 @@ Module Type Ctr.
 Parameter create : ctr unit.
 Parameter incr : unit -> ctr unit.
 Parameter get : unit -> ctr CoqBigInt.t. (*Important - in state monad*)
+
+Parameter st_spec_get: forall (P1: CoqBigInt.t -> Prop) 
+  (Q1: CoqBigInt.t -> CoqBigInt.t -> CoqBigInt.t -> Prop),
+  (forall i, P1 i -> Q1 i i i) ->
+  st_spec P1 (get tt) Q1.
+
+Parameter st_spec_incr: forall (P1: CoqBigInt.t -> Prop) 
+  (Q1: CoqBigInt.t -> unit -> CoqBigInt.t -> Prop),
+  (forall i, P1 i -> Q1 i tt (CoqBigInt.succ i)) ->
+  st_spec P1 (incr tt) Q1.
+
 End Ctr.
 
 Module Type BigIntVal.
@@ -28,4 +39,22 @@ Definition incr (_: unit) : ctr unit :=
   i <- St.get tt ;;
   St.set (CoqBigInt.succ i).
 Definition get (_: unit) : ctr CoqBigInt.t := St.get tt.
+
+Lemma st_spec_get (P1: CoqBigInt.t -> Prop) 
+  (Q1: CoqBigInt.t -> CoqBigInt.t -> CoqBigInt.t -> Prop):
+  (forall i, P1 i -> Q1 i i i) ->
+  st_spec P1 (get tt) Q1.
+Proof.
+  apply st_spec_get. (*need because Coq cannot unify*)
+Qed.
+
+Lemma st_spec_incr (P1: CoqBigInt.t -> Prop) 
+  (Q1: CoqBigInt.t -> unit -> CoqBigInt.t -> Prop):
+  (forall i, P1 i -> Q1 i tt (CoqBigInt.succ i)) ->
+  st_spec P1 (incr tt) Q1.
+Proof.
+  intros Hsucc. unfold st_spec; simpl. auto.
+Qed.
+
+
 End MakeCtr.
